Merge the "..._has_pre" and well-formness predicate

fstar/MLS.Symbolic.Parsers.fst
@@ -6,7 +6,6 @@ open MLS.NetworkTypes
 open MLS.TreeSync.NetworkTypes
 open MLS.TreeSync.Types
 open MLS.TreeSync.Invariants.AuthService
-open MLS.TreeSync.Symbolic.IsValid
 
 #set-options "--fuel 1 --ifuel 1"
 
@@ -54,15 +53,52 @@ val ps_treesync: #bytes:Type0 -> {|bytes_like bytes|} -> tkt:treekem_types bytes
 let ps_treesync #bytes tkt l i =
   ps_tree (ps_option (ps_leaf_node_nt tkt)) (ps_option (ps_parent_node_nt tkt)) l i
 
-val ps_treesync_is_well_formed: #bytes:Type0 -> {|bytes_like bytes|} -> tkt:treekem_types bytes -> l:nat -> i:tree_index l -> pre:bytes_compatible_pre bytes -> x:treesync bytes tkt l i -> Lemma
-  (is_well_formed_partial (ps_treesync tkt l i) pre x <==> treesync_has_pre pre x)
-let rec ps_treesync_is_well_formed #bytes #bl tkt l i pre x =
-  match x with
-  | TLeaf _ -> ()
-  | TNode data left right ->
-    ps_treesync_is_well_formed tkt (l-1) (left_index i) pre left;
-    ps_treesync_is_well_formed tkt (l-1) (right_index i) pre right
-
 val ps_as_tokens: #bytes:Type0 -> {|bytes_like bytes|} -> #as_token:Type0 -> parser_serializer bytes as_token -> l:nat -> i:tree_index l -> parser_serializer bytes (as_tokens bytes as_token l i)
 let ps_as_tokens #bytes #bl #as_token ps_token l i =
   ps_tree (ps_option ps_token) ps_unit l i
+
+noeq type path_internal_node (bytes:Type0) {|bytes_like bytes|} (leaf_t:Type0) (node_t:Type0) (l:pos) (i:tree_index l) (li:leaf_index l i) (ps_node_t:parser_serializer_unit bytes node_t) (ps_next:parser_serializer bytes (path leaf_t node_t (l-1) (if is_left_leaf li then left_index i else right_index i) li)) = {
+  [@@@ with_parser #bytes ps_node_t]
+  data: node_t;
+  [@@@ with_parser #bytes ps_next]
+  next: path leaf_t node_t (l-1) (if is_left_leaf li then left_index i else right_index i) li;
+}
+
+%splice [ps_path_internal_node] (gen_parser (`path_internal_node))
+%splice [ps_path_internal_node_is_well_formed] (gen_is_well_formed_lemma (`path_internal_node))
+
+[@@"opaque_to_smt"]
+val ps_path: #bytes:Type0 -> {|bytes_like bytes|} -> #leaf_t:Type0 -> #node_t:Type0 -> parser_serializer bytes leaf_t -> parser_serializer_unit bytes node_t -> l:nat -> i:tree_index l -> li:leaf_index l i -> parser_serializer bytes (path leaf_t node_t l i li)
+let rec ps_path #bytes #bl #leaf_t #node_t ps_leaf_t ps_node_t l i li =
+  if l = 0 then (
+    mk_isomorphism
+      (path leaf_t node_t 0 i li)
+      ps_leaf_t
+      (fun x -> PLeaf x)
+      (fun (PLeaf x) -> x)
+  ) else (
+    mk_isomorphism
+      (path leaf_t node_t l i li)
+      (ps_path_internal_node #bytes #bl leaf_t node_t l i li ps_node_t (ps_path ps_leaf_t ps_node_t (l-1) (if is_left_leaf li then left_index i else right_index i) li))
+      (fun {data; next} -> PNode data next)
+      (fun (PNode data next) -> {data; next;})
+  )
+
+val ps_path_is_well_formed: #bytes:Type0 -> {|bytes_like bytes|} -> #leaf_t:Type0 -> #node_t:Type0 -> ps_leaf_t:parser_serializer bytes leaf_t -> ps_node_t:parser_serializer_unit bytes node_t -> l:nat -> i:tree_index l -> li:leaf_index l i -> pre:bytes_compatible_pre bytes -> x:path leaf_t node_t l i li -> Lemma
+  (is_well_formed_partial (ps_path ps_leaf_t ps_node_t l i li) pre x <==> (
+    match x with
+    | PLeaf y -> is_well_formed_partial ps_leaf_t pre y
+    | PNode y next -> is_well_formed_partial ps_node_t pre y /\ is_well_formed_partial (ps_path ps_leaf_t ps_node_t (l-1) (if is_left_leaf li then left_index i else right_index i) li) pre next
+  ))
+  [SMTPat (is_well_formed_partial (ps_path ps_leaf_t ps_node_t l i li) pre x)]
+let ps_path_is_well_formed #bytes #bl #leaf_t #node_t ps_leaf_t ps_node_t l i li pre x =
+  // For some reason, reveal_opaque doesn't work here
+  normalize_term_spec (ps_path ps_leaf_t ps_node_t l i li)
+
+val ps_pathsync: #bytes:Type0 -> {|bytes_like bytes|} -> tkt:treekem_types bytes -> l:nat -> i:tree_index l -> li:leaf_index l i -> parser_serializer bytes (pathsync bytes tkt l i li)
+let ps_pathsync #bytes tkt l i li =
+  ps_path (ps_leaf_node_nt tkt) (ps_option tkt.ps_node_content) l i li
+
+val ps_external_pathsync: #bytes:Type0 -> {|bytes_like bytes|} -> tkt:treekem_types bytes -> l:nat -> i:tree_index l -> li:leaf_index l i -> parser_serializer bytes (external_pathsync bytes tkt l i li)
+let ps_external_pathsync #bytes tkt l i li =
+  ps_path (ps_leaf_node_data_nt tkt) (ps_option tkt.ps_node_content) l i li
